Comparisons.v
@@ -1,0 +1,36 @@
+
+From Coq Require Import List.
+Import ListNotations.
+
+(** * Some complements on [comparison] *)
+
+Set Implicit Arguments.
+
+(** A notation for lexicographic comparison.
+    Note that [c2] might not need to be evaluated (lazyness). *)
+
+Notation "c1 >>= c2" :=
+  (match c1 with Lt => Lt | Gt => Gt | Eq => c2 end) (at level 70).
+
+(** Lexicographic comparison on pairs *)
+
+Section PairComp.
+Variable A B : Type.
+Variable cmpA : A -> A -> comparison.
+Variable cmpB : B -> B -> comparison.
+Definition pair_compare '(a,b) '(a',b') := cmpA a a' >>= cmpB b b'.
+End PairComp.
+
+(** Comparison on lists *)
+
+Section ListComp.
+Variable A : Type.
+Variable cmp : A -> A -> comparison.
+Fixpoint list_compare (l1 l2 : list A) :=
+  match l1, l2 with
+  | [], [] => Eq
+  | [], _ => Lt
+  | _, [] => Gt
+  | x1::l1', x2::l2' => cmp x1 x2 >>= list_compare l1' l2'
+  end.
+End ListComp.
